November report (#149)
* Refactoring reset_traces to full replays

* Initial draft for the report

* Common Futures report.

* Add liveness section to report

* add strictorder refactoring and proof movies to report

Co-authored-by: mcalancea <mihai.calancea@gmail.com>
Co-authored-by: Brandon Moore <brandon.moore@runtimeverification.com>
Co-authored-by: Karl Palmskog <palmskog@gmail.com>

VLSM/Equivocators/Composition/SimulatingFree/FullReplayTraces.v
@@ -105,67 +105,67 @@ Definition spawn_initial_state
   : vaction equivocators_no_equivocations_vlsm
   := map (initial_new_machine_transition_item is) index_listing.
 
-Definition equivocate_trace_from
-  (reset_state : vstate equivocators_no_equivocations_vlsm)
+Definition replay_trace_from
+  (full_replay_state : vstate equivocators_no_equivocations_vlsm)
   (is : vstate equivocators_no_equivocations_vlsm)
   (tr : list (vtransition_item equivocators_no_equivocations_vlsm))
   : list (vtransition_item equivocators_no_equivocations_vlsm)
   :=
   let initial := spawn_initial_state is in
-  let reindex := map (update_euivocators_transition_item_descriptor reset_state) tr in
-  fst (apply_action equivocators_no_equivocations_vlsm reset_state (initial ++ reindex)).
+  let reindex := map (update_euivocators_transition_item_descriptor full_replay_state) tr in
+  fst (apply_action equivocators_no_equivocations_vlsm full_replay_state (initial ++ reindex)).
 
-Lemma equivocate_trace_from_app
-  (reset_state : vstate equivocators_no_equivocations_vlsm)
+Lemma replay_trace_from_app
+  (full_replay_state : vstate equivocators_no_equivocations_vlsm)
   (is : vstate equivocators_no_equivocations_vlsm)
   (tra trb : list (vtransition_item equivocators_no_equivocations_vlsm))
-  (eqva := equivocate_trace_from reset_state is tra)
-  (lsta := last (map destination eqva) reset_state)
-  : equivocate_trace_from reset_state is (tra ++ trb) =
+  (eqva := replay_trace_from full_replay_state is tra)
+  (lsta := last (map destination eqva) full_replay_state)
+  : replay_trace_from full_replay_state is (tra ++ trb) =
     eqva ++
     fst
       (apply_action equivocators_no_equivocations_vlsm lsta
-        (map (update_euivocators_transition_item_descriptor reset_state) trb)
+        (map (update_euivocators_transition_item_descriptor full_replay_state) trb)
       ).
 Proof.
   unfold lsta, eqva. clear lsta eqva.
-  unfold equivocate_trace_from in *.
+  unfold replay_trace_from in *.
   rewrite map_app at 1.
   rewrite app_assoc.
   rewrite apply_action_app at 1.
   destruct
-    (apply_action equivocators_no_equivocations_vlsm reset_state
-      (spawn_initial_state is ++ map (update_euivocators_transition_item_descriptor reset_state) tra)
+    (apply_action equivocators_no_equivocations_vlsm full_replay_state
+      (spawn_initial_state is ++ map (update_euivocators_transition_item_descriptor full_replay_state) tra)
     ) as (tra_items, tra_final) eqn:Htra.
   unfold fst at 2. unfold fst at 3.
   specialize
-    (apply_action_last equivocators_no_equivocations_vlsm reset_state
+    (apply_action_last equivocators_no_equivocations_vlsm full_replay_state
       (spawn_initial_state is ++
-        map (update_euivocators_transition_item_descriptor reset_state) tra)
+        map (update_euivocators_transition_item_descriptor full_replay_state) tra)
     ) as Hlst.
   rewrite Htra in Hlst. simpl in Hlst.
   simpl. rewrite Hlst. simpl.
   destruct
     (apply_action equivocators_no_equivocations_vlsm tra_final
-      (map (update_euivocators_transition_item_descriptor reset_state) trb))
+      (map (update_euivocators_transition_item_descriptor full_replay_state) trb))
     as (trb_items, trb_final).
   reflexivity.
 Qed.
 
-Lemma apply_action_reset_state_initial_state
-  (reset_state : vstate equivocators_no_equivocations_vlsm)
+Lemma apply_action_full_replay_state_initial_state
+  (full_replay_state : vstate equivocators_no_equivocations_vlsm)
   (is : vstate equivocators_no_equivocations_vlsm)
-  (tr_reset_is :=
-    apply_action equivocators_no_equivocations_vlsm reset_state
+  (tr_full_replay_is :=
+    apply_action equivocators_no_equivocations_vlsm full_replay_state
       (spawn_initial_state is)
   )
   (eqv : equiv_index)
-  : snd tr_reset_is (eqv)
+  : snd tr_full_replay_is (eqv)
   = equivocator_state_extend (IM (eqv))
-    (reset_state (eqv))
+    (full_replay_state (eqv))
     (projT2 (is (eqv)) (of_nat_lt (Hzero (IM (eqv)) (is (eqv))))).
 Proof.
-  unfold spawn_initial_state in tr_reset_is.
+  unfold spawn_initial_state in tr_full_replay_is.
   assert
     (Heq_state_not_in :
       forall
@@ -206,11 +206,11 @@ Proof.
         (Hnodup : NoDup l)
         (Heqv : In eqv l),
         snd
-          (apply_action equivocators_no_equivocations_vlsm reset_state
+          (apply_action equivocators_no_equivocations_vlsm full_replay_state
             (map (initial_new_machine_transition_item is) l))
           (eqv)
         = equivocator_state_extend (IM (eqv))
-          (reset_state (eqv))
+          (full_replay_state (eqv))
           (projT2 (is (eqv)) (of_nat_lt (Hzero (IM (eqv)) (is (eqv)))))
     ).
   { intros. apply in_split in Heqv as Heqv.
@@ -223,9 +223,9 @@ Proof.
     specialize (Heq_state_not_in pref) as Hpref.
     spec Hpref.
     { intro contra. elim Heqv. apply in_app_iff. left. assumption. }
-    spec Hpref reset_state.
+    spec Hpref full_replay_state.
     destruct
-      (apply_action equivocators_no_equivocations_vlsm reset_state
+      (apply_action equivocators_no_equivocations_vlsm full_replay_state
         (map (initial_new_machine_transition_item is) pref))
       as (pref_items, pref_final).
     simpl in Hpref.
@@ -251,8 +251,8 @@ Proof.
   apply Heq_state_in. apply (proj1 finite_index). apply (proj2 finite_index).
 Qed.
 
-Lemma equivocate_trace_from_state_correspondence'
-  (reset_state : vstate equivocators_no_equivocations_vlsm)
+Lemma replay_trace_from_state_correspondence'
+  (full_replay_state : vstate equivocators_no_equivocations_vlsm)
   (is : vstate equivocators_no_equivocations_vlsm)
   (His : vinitial_state_prop equivocators_no_equivocations_vlsm is)
   (epref : list (vtransition_item equivocators_no_equivocations_vlsm))
@@ -260,35 +260,35 @@ Lemma equivocate_trace_from_state_correspondence'
     apply_action equivocators_no_equivocations_vlsm is
       (trace_to_action equivocators_no_equivocations_vlsm epref)
   )
-  (tr_reset_is_epref :=
-    apply_action equivocators_no_equivocations_vlsm reset_state
+  (tr_full_replay_is_epref :=
+    apply_action equivocators_no_equivocations_vlsm full_replay_state
       (spawn_initial_state is
-      ++ map (update_euivocators_transition_item_descriptor reset_state) epref)
+      ++ map (update_euivocators_transition_item_descriptor full_replay_state) epref)
   )
   (eqv : equiv_index)
-  : S (projT1 (snd tr_is_epref (eqv))) + S (projT1 (reset_state (eqv))) = S (projT1 (snd tr_reset_is_epref (eqv)))
-  /\ (epref <> [] -> option_map output (last_error (fst tr_is_epref)) = option_map output (last_error (fst tr_reset_is_epref)))
+  : S (projT1 (snd tr_is_epref (eqv))) + S (projT1 (full_replay_state (eqv))) = S (projT1 (snd tr_full_replay_is_epref (eqv)))
+  /\ (epref <> [] -> option_map output (last_error (fst tr_is_epref)) = option_map output (last_error (fst tr_full_replay_is_epref)))
   /\ (forall
     (id : nat)
     (Hid: id < S (projT1 (snd tr_is_epref (eqv)))),
     exists
-    (Hi : id + S (projT1 (reset_state (eqv))) < S (projT1 (snd tr_reset_is_epref (eqv)))),
+    (Hi : id + S (projT1 (full_replay_state (eqv))) < S (projT1 (snd tr_full_replay_is_epref (eqv)))),
     projT2 (snd tr_is_epref (eqv)) (of_nat_lt Hid) =
-    projT2 (snd tr_reset_is_epref (eqv)) (of_nat_lt Hi))
+    projT2 (snd tr_full_replay_is_epref (eqv)) (of_nat_lt Hi))
   /\ forall
     (id : nat)
-    (Hid: id < S (projT1 (reset_state (eqv)))),
+    (Hid: id < S (projT1 (full_replay_state (eqv)))),
     exists
-    (Hi : id < S (projT1 (snd tr_reset_is_epref (eqv)))),
-    projT2 (snd tr_reset_is_epref (eqv)) (of_nat_lt Hi) =
-    projT2 (reset_state (eqv)) (of_nat_lt Hid) .
+    (Hi : id < S (projT1 (snd tr_full_replay_is_epref (eqv)))),
+    projT2 (snd tr_full_replay_is_epref (eqv)) (of_nat_lt Hi) =
+    projT2 (full_replay_state (eqv)) (of_nat_lt Hid) .
 Proof.
   generalize dependent eqv.
   induction epref using rev_ind; intros.
-  - simpl in *. clear tr_is_epref. unfold tr_reset_is_epref. clear tr_reset_is_epref.
+  - simpl in *. clear tr_is_epref. unfold tr_full_replay_is_epref. clear tr_full_replay_is_epref.
     rewrite app_nil_r.
-    rewrite apply_action_reset_state_initial_state.
-    destruct (reset_state (eqv)) as (neqv, seqv).
+    rewrite apply_action_full_replay_state_initial_state.
+    destruct (full_replay_state (eqv)) as (neqv, seqv).
     unfold equivocator_state_extend. simpl.
     specialize (equivocators_initial_state_size IM Hbs i0 _ _ is His eqv) as His_size.
     split; [rewrite His_size; reflexivity|].
@@ -326,32 +326,32 @@ Proof.
     simpl in IHepref.
     remember
       (apply_action equivocators_no_equivocations_vlsm
-      reset_state
+      full_replay_state
       (spawn_initial_state is ++
        map
          (update_euivocators_transition_item_descriptor
-            reset_state) (epref ++ [x])))
-      as tr_reset_is_epref'.
-    unfold tr_reset_is_epref in *. clear tr_reset_is_epref.
-    rewrite map_app in Heqtr_reset_is_epref'.
-    rewrite app_assoc in Heqtr_reset_is_epref'.
-    rewrite apply_action_app in Heqtr_reset_is_epref'.
+            full_replay_state) (epref ++ [x])))
+      as tr_full_replay_is_epref'.
+    unfold tr_full_replay_is_epref in *. clear tr_full_replay_is_epref.
+    rewrite map_app in Heqtr_full_replay_is_epref'.
+    rewrite app_assoc in Heqtr_full_replay_is_epref'.
+    rewrite apply_action_app in Heqtr_full_replay_is_epref'.
     remember
       (apply_action equivocators_no_equivocations_vlsm
-      reset_state
+      full_replay_state
       (spawn_initial_state is ++
        map
          (update_euivocators_transition_item_descriptor
-            reset_state) epref))
-      as tr_reset_is_epref.
-    destruct tr_reset_is_epref as (reset_is_epref_items, reset_is_epref_final).
+            full_replay_state) epref))
+      as tr_full_replay_is_epref.
+    destruct tr_full_replay_is_epref as (full_replay_is_epref_items, full_replay_is_epref_final).
     unfold apply_action in Heqtr_is_epref'. simpl in Heqtr_is_epref'.
-    unfold apply_action in Heqtr_reset_is_epref'. simpl in Heqtr_reset_is_epref'.
-    destruct x. simpl in Heqtr_reset_is_epref'. simpl in Heqtr_is_epref'.
+    unfold apply_action in Heqtr_full_replay_is_epref'. simpl in Heqtr_full_replay_is_epref'.
+    destruct x. simpl in Heqtr_full_replay_is_epref'. simpl in Heqtr_is_epref'.
     destruct l as (eqv', l).
     destruct l as (l, d).
     destruct d as [sd | id' fd'].
-    + simpl in Heqtr_reset_is_epref'. simpl in Heqtr_is_epref'.
+    + simpl in Heqtr_full_replay_is_epref'. simpl in Heqtr_is_epref'.
       subst. simpl in *.
       destruct (decide (eqv = eqv')).
       * subst eqv'.
@@ -366,24 +366,24 @@ Proof.
         destruct (epref_final (eqv)) as (nepref_eqv, sepref_eqv) eqn:Hepref_final_eqv.
         simpl in IHepref. subst stat. simpl.
         unfold equivocator_state_extend.
-        destruct (reset_is_epref_final (eqv)) as (nreset_is_epref_eqv, sreset_is_epref_eqv).
+        destruct (full_replay_is_epref_final (eqv)) as (nfull_replay_is_epref_eqv, sfull_replay_is_epref_eqv).
         unfold projT1. unfold projT2.
         simpl in IHepref.
-        destruct (reset_state (eqv)) as (nreset_state_eqv, sreset_state_eqv) eqn:Hreset_state_eqv.
+        destruct (full_replay_state (eqv)) as (nfull_replay_state_eqv, sfull_replay_state_eqv) eqn:Hfull_replay_state_eqv.
         simpl in IHepref.
         destruct IHepref as [Hsize Hstate].
         split; [congruence|].
         repeat split.
         -- intros. repeat rewrite last_error_is_last. reflexivity.
         -- intros.
-          assert (Hi : id + S nreset_state_eqv < S (S nreset_is_epref_eqv)) by lia.
+          assert (Hi : id + S nfull_replay_state_eqv < S (S nfull_replay_is_epref_eqv)) by lia.
           exists Hi.
           repeat rewrite to_nat_of_nat.
           destruct (nat_eq_dec id (S nepref_eqv)).
           ++ subst id.
-            destruct (nat_eq_dec (S nepref_eqv + S nreset_state_eqv) (S nreset_is_epref_eqv))
+            destruct (nat_eq_dec (S nepref_eqv + S nfull_replay_state_eqv) (S nfull_replay_is_epref_eqv))
             ; [reflexivity|lia].
-          ++ destruct (nat_eq_dec (id + S nreset_state_eqv) (S nreset_is_epref_eqv) ) ; [lia|].
+          ++ destruct (nat_eq_dec (id + S nfull_replay_state_eqv) (S nfull_replay_is_epref_eqv) ) ; [lia|].
             assert (Hid' : id < S nepref_eqv) by lia.
             destruct Hstate as [_ [Hstate _]].
             spec Hstate  id Hid'.
@@ -394,41 +394,41 @@ Proof.
             destruct Hstate as [Hi' Hstate].
             rewrite Hstate. f_equal. apply of_nat_ext.
         -- intros.
-          assert (Hi : id < S (S nreset_is_epref_eqv)) by lia.
+          assert (Hi : id < S (S nfull_replay_is_epref_eqv)) by lia.
           exists Hi. rewrite to_nat_of_nat.
-          destruct (nat_eq_dec id (S nreset_is_epref_eqv)); [lia|].
+          destruct (nat_eq_dec id (S nfull_replay_is_epref_eqv)); [lia|].
           destruct Hstate as [_ [_ Hstate]].
           spec Hstate id Hid.
           destruct Hstate as [Hi' Hstate].
           rewrite <- Hstate. f_equal. apply of_nat_ext.
       * remember
-          (state_update (Common.equivocator_IM IM) reset_is_epref_final
+          (state_update (Common.equivocator_IM IM) full_replay_is_epref_final
           (eqv')
           (equivocator_state_extend (IM (eqv'))
-             (reset_is_epref_final (eqv')) sd) (eqv))
+             (full_replay_is_epref_final (eqv')) sd) (eqv))
           as stat.
         spec IHepref eqv.
         rewrite state_update_neq in Heqstat by assumption.
         rewrite state_update_neq by assumption.
         destruct (epref_final (eqv)) as (nepref_eqv, sepref_eqv) eqn:Hepref_final_eqv.
         simpl in IHepref. subst stat. simpl.
-        destruct (reset_is_epref_final (eqv)) as (nreset_is_epref_eqv, sreset_is_epref_eqv).
+        destruct (full_replay_is_epref_final (eqv)) as (nfull_replay_is_epref_eqv, sfull_replay_is_epref_eqv).
         unfold projT1. unfold projT2.
         simpl in IHepref.
-        destruct (reset_state (eqv)) as (nreset_state_eqv, sreset_state_eqv) eqn:Hreset_state_eqv.
+        destruct (full_replay_state (eqv)) as (nfull_replay_state_eqv, sfull_replay_state_eqv) eqn:Hfull_replay_state_eqv.
         simpl in IHepref.
         destruct IHepref as [Hsize [_ Hstate]].
         split; [congruence|].
         split; [|assumption].
         intros. repeat rewrite last_error_is_last. reflexivity.
-    + unfold vtransition in Heqtr_reset_is_epref'. simpl in Heqtr_reset_is_epref'.
-      unfold vtransition in Heqtr_reset_is_epref'.
-      match type of Heqtr_reset_is_epref' with
+    + unfold vtransition in Heqtr_full_replay_is_epref'. simpl in Heqtr_full_replay_is_epref'.
+      unfold vtransition in Heqtr_full_replay_is_epref'.
+      match type of Heqtr_full_replay_is_epref' with
       | _ = let (_, _) := let (_, _) := let (_, _) := let (_, _) := ?t 
-            in _ in _ in _ in _ => remember t as t_reset_is_epref'
+            in _ in _ in _ in _ => remember t as t_full_replay_is_epref'
       end.
-      unfold_transition Heqt_reset_is_epref'.
-      unfold snd in Heqt_reset_is_epref'.
+      unfold_transition Heqt_full_replay_is_epref'.
+      unfold snd in Heqt_full_replay_is_epref'.
       unfold vtransition in Heqtr_is_epref'.
       simpl in Heqtr_is_epref'.
       match type of Heqtr_is_epref' with
@@ -442,15 +442,15 @@ Proof.
       specialize (IHepref eqv') as IHepref'.
       specialize (IHepref eqv).
       destruct (epref_final (eqv')) as (nepref_eqv', sepref_eqv') eqn:Hepref_final_eqv'.
-      destruct (reset_is_epref_final (eqv')) as (nreset_is_epref_eqv', sreset_is_epref_eqv') eqn:Hreset_is_epref_eqv'.
-      destruct (reset_state (eqv')) as (nreset_state_eqv', sreset_state_eqv') eqn:Hreset_state_eqv'.
+      destruct (full_replay_is_epref_final (eqv')) as (nfull_replay_is_epref_eqv', sfull_replay_is_epref_eqv') eqn:Hfull_replay_is_epref_eqv'.
+      destruct (full_replay_state (eqv')) as (nfull_replay_state_eqv', sfull_replay_state_eqv') eqn:Hfull_replay_state_eqv'.
       unfold projT1 in Heqt_is_epref'. unfold projT2 in Heqt_is_epref'.
-      unfold projT1 in Heqt_reset_is_epref'. unfold projT2 in Heqt_reset_is_epref'.
-      unfold projT1 in Heqtr_reset_is_epref'.
+      unfold projT1 in Heqt_full_replay_is_epref'. unfold projT2 in Heqt_full_replay_is_epref'.
+      unfold projT1 in Heqtr_full_replay_is_epref'.
       simpl in IHepref'.
       destruct IHepref' as [Hsize' Hstate'].
       destruct (le_lt_dec (S nepref_eqv') id').
-      * destruct (le_lt_dec (S nreset_is_epref_eqv') (id' + S nreset_state_eqv'))
+      * destruct (le_lt_dec (S nfull_replay_is_epref_eqv') (id' + S nfull_replay_state_eqv'))
         ; [|lia].
         subst. simpl.
         destruct (decide (eqv = eqv')).
@@ -461,9 +461,9 @@ Proof.
           rewrite state_update_eq in Heqstat.
           rewrite state_update_eq.
           subst.
-          rewrite Hreset_is_epref_eqv' in *.
+          rewrite Hfull_replay_is_epref_eqv' in *.
           rewrite Hepref_final_eqv' in *.
-          rewrite Hreset_state_eqv' in *.
+          rewrite Hfull_replay_state_eqv' in *.
           simpl in IHepref.
           unfold projT1. unfold projT2.
           destruct Hstate' as [_ Hstate'].
@@ -478,13 +478,13 @@ Proof.
           rewrite state_update_neq by assumption.
           destruct (epref_final (eqv)) as (nepref_eqv, sepref_eqv) eqn:Hepref_final_eqv.
           simpl in IHepref. subst stat. simpl.
-          destruct (reset_is_epref_final (eqv)) as (nreset_is_epref_eqv, sreset_is_epref_eqv).
-          destruct (reset_state (eqv)) as (nreset_state_eqv, sreset_state_eqv) eqn:Hreset_state_eqv.
+          destruct (full_replay_is_epref_final (eqv)) as (nfull_replay_is_epref_eqv, sfull_replay_is_epref_eqv).
+          destruct (full_replay_state (eqv)) as (nfull_replay_state_eqv, sfull_replay_state_eqv) eqn:Hfull_replay_state_eqv.
           unfold projT1. unfold projT2.
           simpl in IHepref. destruct IHepref as [Hsize [_ Heq]].
           split; [assumption|]. split; [|assumption].
           intros. repeat rewrite last_error_is_last. reflexivity.
-      * destruct (le_lt_dec (S nreset_is_epref_eqv') (id' + S nreset_state_eqv')); [lia|].
+      * destruct (le_lt_dec (S nfull_replay_is_epref_eqv') (id' + S nfull_replay_state_eqv')); [lia|].
         destruct
           (vtransition (IM (eqv'))
           (fst (l, Existing (IM (eqv')) id' fd'))
@@ -495,8 +495,8 @@ Proof.
           (fst
              (l,
              Existing (IM (eqv'))
-               (id' + S nreset_state_eqv') fd'))
-          (sreset_is_epref_eqv'
+               (id' + S nfull_replay_state_eqv') fd'))
+          (sfull_replay_is_epref_eqv'
              (Fin2Restrict.n2f l1), input))
           as (seqv'', omeqv'') eqn:Hteqv''.
         destruct fd' eqn:Hfd'.
@@ -522,9 +522,9 @@ Proof.
             rewrite state_update_eq in Heqstat.
             rewrite state_update_eq.
             subst.
-            rewrite Hreset_is_epref_eqv' in *.
+            rewrite Hfull_replay_is_epref_eqv' in *.
             rewrite Hepref_final_eqv' in *.
-            rewrite Hreset_state_eqv' in *.
+            rewrite Hfull_replay_state_eqv' in *.
             simpl in IHepref.
             simpl.
             destruct IHepref as [Hsize Hstate].
@@ -539,21 +539,21 @@ Proof.
             rewrite Hteqv' in Hteqv''. inversion Hteqv''. subst seqv'' omeqv''.
             split ; [intros; repeat rewrite last_error_is_last; reflexivity|].
             split; intros.
-            ** assert (Hi : id + S nreset_state_eqv' < S (S nreset_is_epref_eqv')) by lia.
+            ** assert (Hi : id + S nfull_replay_state_eqv' < S (S nfull_replay_is_epref_eqv')) by lia.
               exists Hi.
               repeat rewrite to_nat_of_nat.
               destruct (nat_eq_dec id (S nepref_eqv')).
               --- subst.
-                destruct (nat_eq_dec (S nepref_eqv' + S nreset_state_eqv') (S nreset_is_epref_eqv'))
+                destruct (nat_eq_dec (S nepref_eqv' + S nfull_replay_state_eqv') (S nfull_replay_is_epref_eqv'))
                 ; [reflexivity | elim n; assumption].
-              --- destruct (nat_eq_dec (id + S nreset_state_eqv') (S nreset_is_epref_eqv'))
+              --- destruct (nat_eq_dec (id + S nfull_replay_state_eqv') (S nfull_replay_is_epref_eqv'))
                 ; [lia|].
                 specialize (Hstate' _ (Common.equivocator_state_extend_obligation_1 nepref_eqv' id Hid n)).
                 destruct Hstate' as [Hi'' Hstate'].
                 rewrite Hstate'. f_equal. apply of_nat_ext.
-            ** assert (Hi : id < S (S nreset_is_epref_eqv')) by lia.
+            ** assert (Hi : id < S (S nfull_replay_is_epref_eqv')) by lia.
               exists Hi. rewrite to_nat_of_nat.
-              destruct (nat_eq_dec id (S nreset_is_epref_eqv')); [lia|].
+              destruct (nat_eq_dec id (S nfull_replay_is_epref_eqv')); [lia|].
               spec Hstate_pre id Hid.
               destruct Hstate_pre as [Hi'' Hstate_pre].
               rewrite <- Hstate_pre. f_equal. apply of_nat_ext.
@@ -574,8 +574,8 @@ Proof.
             rewrite state_update_neq by assumption.
             destruct (epref_final (eqv)) as (nepref_eqv, sepref_eqv) eqn:Hepref_final_eqv.
             simpl in IHepref. subst stat. simpl.
-            destruct (reset_is_epref_final (eqv)) as (nreset_is_epref_eqv, sreset_is_epref_eqv).
-            destruct (reset_state (eqv)) as (nreset_state_eqv, sreset_state_eqv) eqn:Hreset_state_eqv.
+            destruct (full_replay_is_epref_final (eqv)) as (nfull_replay_is_epref_eqv, sfull_replay_is_epref_eqv).
+            destruct (full_replay_state (eqv)) as (nfull_replay_state_eqv, sfull_replay_state_eqv) eqn:Hfull_replay_state_eqv.
             unfold projT1. unfold projT2.
             simpl in IHepref. destruct IHepref as [Hsize [_ Heq]].
             destruct Hstate' as [_ [Hstate' Hstate_pre]].
@@ -604,9 +604,9 @@ Proof.
             rewrite state_update_eq.
             subst.
             simpl.
-            rewrite Hreset_is_epref_eqv' in *.
+            rewrite Hfull_replay_is_epref_eqv' in *.
             rewrite Hepref_final_eqv' in *.
-            rewrite Hreset_state_eqv' in *.
+            rewrite Hfull_replay_state_eqv' in *.
             simpl in IHepref.
             simpl.
             destruct IHepref as [Hsize Hstate].
@@ -621,7 +621,7 @@ Proof.
             rewrite Hteqv' in Hteqv''. inversion Hteqv''. subst seqv'' omeqv''.
             split; [intros; repeat rewrite last_error_is_last; reflexivity|].
             split; intros.
-            ** assert (Hi : id + S nreset_state_eqv' < S nreset_is_epref_eqv') by lia.
+            ** assert (Hi : id + S nfull_replay_state_eqv' < S nfull_replay_is_epref_eqv') by lia.
               exists Hi.
               destruct (nat_eq_dec id id').
               --- subst id'.
@@ -653,7 +653,7 @@ Proof.
                 spec Hstate' id Hid.
                 destruct Hstate' as [Hi' Hstate'].
                 rewrite Hstate'. f_equal. apply of_nat_ext.
-            ** assert (Hi : id < S nreset_is_epref_eqv') by lia.
+            ** assert (Hi : id < S nfull_replay_is_epref_eqv') by lia.
               exists Hi.
               specialize (Hstate_pre id Hid).
               destruct Hstate_pre as [Hi'' Hstate_pre].
@@ -673,8 +673,8 @@ Proof.
             rewrite state_update_neq by assumption.
             destruct (epref_final (eqv)) as (nepref_eqv, sepref_eqv) eqn:Hepref_final_eqv.
             simpl in IHepref. subst stat. simpl.
-            destruct (reset_is_epref_final (eqv)) as (nreset_is_epref_eqv, sreset_is_epref_eqv).
-            destruct (reset_state (eqv)) as (nreset_state_eqv, sreset_state_eqv) eqn:Hreset_state_eqv.
+            destruct (full_replay_is_epref_final (eqv)) as (nfull_replay_is_epref_eqv, sfull_replay_is_epref_eqv).
+            destruct (full_replay_state (eqv)) as (nfull_replay_state_eqv, sfull_replay_state_eqv) eqn:Hfull_replay_state_eqv.
             unfold projT1. unfold projT2.
             unfold fst in Hteqv'. unfold fst in Hteqv''.
             destruct Hstate' as [_ [Hstate' Hstate_pre]].
@@ -690,45 +690,45 @@ Proof.
             intros. repeat rewrite last_error_is_last. reflexivity.
 Qed.
 
-Lemma equivocate_trace_from_state_correspondence
-  (reset_state : vstate equivocators_no_equivocations_vlsm)
+Lemma replay_trace_from_state_correspondence
+  (full_replay_state : vstate equivocators_no_equivocations_vlsm)
   (is : vstate equivocators_no_equivocations_vlsm)
   (His : vinitial_state_prop equivocators_no_equivocations_vlsm is)
   (tr : list (vtransition_item equivocators_no_equivocations_vlsm))
   (Htr : finite_protocol_trace_from equivocators_no_equivocations_vlsm is tr)
   (last_is_tr := last (map destination tr) is)
-  (tr_reset_is_tr := equivocate_trace_from reset_state is tr)
-  (last_reset_is_tr := last (map destination tr_reset_is_tr) reset_state)
-  : (tr <> [] -> option_map output (last_error tr) = option_map output (last_error tr_reset_is_tr))
+  (tr_full_replay_is_tr := replay_trace_from full_replay_state is tr)
+  (last_full_replay_is_tr := last (map destination tr_full_replay_is_tr) full_replay_state)
+  : (tr <> [] -> option_map output (last_error tr) = option_map output (last_error tr_full_replay_is_tr))
   /\ forall
     (eqv : equiv_index),
-  S (projT1 (last_is_tr (eqv))) + S (projT1 (reset_state (eqv))) = S (projT1 (last_reset_is_tr (eqv)))
+  S (projT1 (last_is_tr (eqv))) + S (projT1 (full_replay_state (eqv))) = S (projT1 (last_full_replay_is_tr (eqv)))
   /\ (forall
     (id : nat)
     (Hid: id < S (projT1 (last_is_tr (eqv)))),
     exists
-    (Hi : id + S (projT1 (reset_state (eqv))) < S (projT1 (last_reset_is_tr (eqv)))),
+    (Hi : id + S (projT1 (full_replay_state (eqv))) < S (projT1 (last_full_replay_is_tr (eqv)))),
     projT2 (last_is_tr (eqv)) (of_nat_lt Hid) =
-    projT2 (last_reset_is_tr (eqv)) (of_nat_lt Hi))
+    projT2 (last_full_replay_is_tr (eqv)) (of_nat_lt Hi))
   /\ forall
     (id : nat)
-    (Hid: id < S (projT1 (reset_state (eqv)))),
+    (Hid: id < S (projT1 (full_replay_state (eqv)))),
     exists
-    (Hi : id < S (projT1 (last_reset_is_tr (eqv)))),
-    projT2 (last_reset_is_tr (eqv)) (of_nat_lt Hi) =
-    projT2 (reset_state (eqv)) (of_nat_lt Hid) .
+    (Hi : id < S (projT1 (last_full_replay_is_tr (eqv)))),
+    projT2 (last_full_replay_is_tr (eqv)) (of_nat_lt Hi) =
+    projT2 (full_replay_state (eqv)) (of_nat_lt Hid) .
 Proof.
   split.
   - set (eqv0 := i0).
     destruct
-      (equivocate_trace_from_state_correspondence'
-        reset_state _ His tr eqv0
+      (replay_trace_from_state_correspondence'
+        full_replay_state _ His tr eqv0
       ) as [_ [Houtput _]].
     rewrite trace_to_action_to_trace in Houtput; assumption.
   - intro eqv.
     specialize
-      (equivocate_trace_from_state_correspondence'
-        reset_state _ His tr eqv
+      (replay_trace_from_state_correspondence'
+        full_replay_state _ His tr eqv
       ) as Hcorrespondence.
     repeat rewrite <- apply_action_last in Hcorrespondence.
     rewrite trace_to_action_to_trace in Hcorrespondence by assumption.
@@ -736,25 +736,25 @@ Proof.
     split; assumption.
 Qed.
 
-Lemma equivocate_trace_from_reset_state_project
-  (reset_state : vstate equivocators_no_equivocations_vlsm)
+Lemma replay_trace_from_full_replay_state_project
+  (full_replay_state : vstate equivocators_no_equivocations_vlsm)
   (is : vstate equivocators_no_equivocations_vlsm)
   (His : vinitial_state_prop equivocators_no_equivocations_vlsm is)
   (tr : list (vtransition_item equivocators_no_equivocations_vlsm))
   (Htr : finite_protocol_trace_from equivocators_no_equivocations_vlsm is tr)
-  (tr_reset_is_tr := equivocate_trace_from reset_state is tr)
-  (last_reset_is_tr := last (map destination tr_reset_is_tr) reset_state)
+  (tr_full_replay_is_tr := replay_trace_from full_replay_state is tr)
+  (last_full_replay_is_tr := last (map destination tr_full_replay_is_tr) full_replay_state)
   (eqv_choice : equivocators_choice)
-  (Heqv_choice : proper_equivocators_choice eqv_choice reset_state)
-  : proper_equivocators_choice eqv_choice last_reset_is_tr /\
-    equivocators_state_project eqv_choice last_reset_is_tr =
-    equivocators_state_project eqv_choice  reset_state.
+  (Heqv_choice : proper_equivocators_choice eqv_choice full_replay_state)
+  : proper_equivocators_choice eqv_choice last_full_replay_is_tr /\
+    equivocators_state_project eqv_choice last_full_replay_is_tr =
+    equivocators_state_project eqv_choice  full_replay_state.
 Proof.
-  assert (Heqv_choice' : proper_equivocators_choice eqv_choice last_reset_is_tr); [|split;[assumption|]].
+  assert (Heqv_choice' : proper_equivocators_choice eqv_choice last_full_replay_is_tr); [|split;[assumption|]].
   - intro eqv. specialize (Heqv_choice eqv). unfold proper_descriptor in *.
     destruct (eqv_choice eqv); [assumption|].
-    destruct (proj2 (equivocate_trace_from_state_correspondence reset_state _ His _ Htr) eqv)
-      as [Hsize _]. unfold last_reset_is_tr. unfold tr_reset_is_tr.
+    destruct (proj2 (replay_trace_from_state_correspondence full_replay_state _ His _ Htr) eqv)
+      as [Hsize _]. unfold last_full_replay_is_tr. unfold tr_full_replay_is_tr.
     lia.
   - apply functional_extensionality_dep_good.
     intros eqv.
@@ -763,19 +763,19 @@ Proof.
     spec Heqv_choice' eqv.
     unfold proper_descriptor in *.
     destruct (eqv_choice eqv); [reflexivity|].
-    destruct (last_reset_is_tr (eqv)) as (last_reset_is_tr_size, last_reset_is_tr_s)
-      eqn:Hlast_reset_is_tr_eqv.
-    destruct (reset_state (eqv)) as (reset_state_size, reset_state_s)
-      eqn:Hreset_state_eqv.
+    destruct (last_full_replay_is_tr (eqv)) as (last_full_replay_is_tr_size, last_full_replay_is_tr_s)
+      eqn:Hlast_full_replay_is_tr_eqv.
+    destruct (full_replay_state (eqv)) as (full_replay_state_size, full_replay_state_s)
+      eqn:Hfull_replay_state_eqv.
     simpl in Heqv_choice, Heqv_choice'.
-    destruct (le_lt_dec (S last_reset_is_tr_size) n); [lia|].
-    destruct (le_lt_dec (S reset_state_size) n); [lia|].
-    destruct (proj2 (equivocate_trace_from_state_correspondence reset_state _ His _ Htr) eqv)
+    destruct (le_lt_dec (S last_full_replay_is_tr_size) n); [lia|].
+    destruct (le_lt_dec (S full_replay_state_size) n); [lia|].
+    destruct (proj2 (replay_trace_from_state_correspondence full_replay_state _ His _ Htr) eqv)
       as [_ [_ Hstate_pre]].
-    rewrite Hreset_state_eqv in Hstate_pre.
+    rewrite Hfull_replay_state_eqv in Hstate_pre.
     specialize (Hstate_pre n Heqv_choice).
-    unfold last_reset_is_tr in *. unfold tr_reset_is_tr in *.
-    rewrite Hlast_reset_is_tr_eqv in Hstate_pre.
+    unfold last_full_replay_is_tr in *. unfold tr_full_replay_is_tr in *.
+    rewrite Hlast_full_replay_is_tr_eqv in Hstate_pre.
     unfold projT1,projT2 in Hstate_pre.
     destruct Hstate_pre as [Hi Hstate_pre].
     replace (of_nat_lt Hi) with (of_nat_lt Heqv_choice') in * by apply of_nat_ext.
@@ -784,9 +784,9 @@ Proof.
     assumption.
 Qed.
 
-Lemma equivocate_trace_from_protocol
-  (reset_state : vstate equivocators_no_equivocations_vlsm)
-  (Hreset_state : protocol_state_prop equivocators_no_equivocations_vlsm reset_state)
+Lemma replay_trace_from_protocol
+  (full_replay_state : vstate equivocators_no_equivocations_vlsm)
+  (Hfull_replay_state : protocol_state_prop equivocators_no_equivocations_vlsm full_replay_state)
   (is : vstate equivocators_no_equivocations_vlsm)
   (tr : list (vtransition_item equivocators_no_equivocations_vlsm))
   (Htr : finite_protocol_trace equivocators_no_equivocations_vlsm is tr)
@@ -813,22 +813,22 @@ Lemma equivocate_trace_from_protocol
         (existT (fun n : index => vlabel (equivocator_IM n))
            (eqv)
            (l0,
-           Existing (IM (eqv)) (id + S (projT1 (reset_state (eqv)))) fd))
+           Existing (IM (eqv)) (id + S (projT1 (full_replay_state (eqv)))) fd))
         (last
            (map Common.destination
               (fst
                  (apply_action (equivocators_constrained_vlsm IM i0 constraint)
-                    reset_state
+                    full_replay_state
                     (spawn_initial_state is ++
                      map
-                       (update_euivocators_transition_item_descriptor reset_state)
-                       epref)))) reset_state, input eitem)
+                       (update_euivocators_transition_item_descriptor full_replay_state)
+                       epref)))) full_replay_state, input eitem)
   )
   : finite_protocol_trace_from (equivocators_constrained_vlsm IM i0 constraint)
-      reset_state (equivocate_trace_from reset_state is tr).
+      full_replay_state (replay_trace_from full_replay_state is tr).
 Proof.
-  assert (Hreset_state' : protocol_state_prop (equivocators_constrained_vlsm IM i0 constraint) reset_state).
-  { destruct Hreset_state as [om Hreset_state]. exists om.
+  assert (Hfull_replay_state' : protocol_state_prop (equivocators_constrained_vlsm IM i0 constraint) full_replay_state).
+  { destruct Hfull_replay_state as [om Hfull_replay_state]. exists om.
     apply (constraint_subsumption_protocol_prop equivocator_IM i0 _ _ Hconstraint_subsumption).
     assumption.
   }
@@ -935,7 +935,7 @@ Proof.
           split.
           ++ simpl. unfold vvalid. simpl.
             specialize
-              (equivocate_trace_from_state_correspondence' reset_state _ (proj2 Htr)
+              (replay_trace_from_state_correspondence' full_replay_state _ (proj2 Htr)
               epref eqv
               )
               as Hstate.
@@ -948,11 +948,11 @@ Proof.
               replace s with
               (projT2
               (snd
-                 (apply_action equivocators_no_equivocations_vlsm reset_state
+                 (apply_action equivocators_no_equivocations_vlsm full_replay_state
                     (spawn_initial_state is ++
                      map
                        (update_euivocators_transition_item_descriptor
-                          reset_state) epref)) (eqv))
+                          full_replay_state) epref)) (eqv))
               (Fin2Restrict.n2f Hi))
             end
             ; [rewrite <- Hstate; assumption|].
@@ -962,39 +962,39 @@ Proof.
             assumption.
 Qed.
 
-Lemma equivocate_trace_from_protocol_free
-  (reset_state : vstate equivocators_no_equivocations_vlsm)
-  (Hreset_state : protocol_state_prop equivocators_no_equivocations_vlsm reset_state)
+Lemma replay_trace_from_protocol_free
+  (full_replay_state : vstate equivocators_no_equivocations_vlsm)
+  (Hfull_replay_state : protocol_state_prop equivocators_no_equivocations_vlsm full_replay_state)
   (is : vstate equivocators_no_equivocations_vlsm)
   (tr : list (vtransition_item equivocators_no_equivocations_vlsm))
   (Htr : finite_protocol_trace equivocators_no_equivocations_vlsm is tr)
   : finite_protocol_trace_from (free_composite_vlsm equivocator_IM i0)
-      reset_state (equivocate_trace_from reset_state is tr).
+      full_replay_state (replay_trace_from full_replay_state is tr).
 Proof.
-  apply equivocate_trace_from_protocol.
+  apply replay_trace_from_protocol.
   - assumption.
   - assumption.
   - intro; intros. exact I.
   - intros. exact I.
 Qed.
 
-Lemma equivocate_trace_from_protocol_equivocating
-  (reset_state : vstate equivocators_no_equivocations_vlsm)
-  (Hreset_state : protocol_state_prop equivocators_no_equivocations_vlsm reset_state)
+Lemma replay_trace_from_protocol_equivocating
+  (full_replay_state : vstate equivocators_no_equivocations_vlsm)
+  (Hfull_replay_state : protocol_state_prop equivocators_no_equivocations_vlsm full_replay_state)
   (is : vstate equivocators_no_equivocations_vlsm)
   (tr : list (vtransition_item equivocators_no_equivocations_vlsm))
   (Htr : finite_protocol_trace equivocators_no_equivocations_vlsm is tr)
   : finite_protocol_trace_from equivocators_no_equivocations_vlsm
-      reset_state (equivocate_trace_from reset_state is tr).
+      full_replay_state (replay_trace_from full_replay_state is tr).
 Proof.
-  apply equivocate_trace_from_protocol
+  apply replay_trace_from_protocol
   ;[assumption|assumption|intro; intros; assumption|].
   intros.
   subst tr.
   destruct Htr as [Htr His].
   apply finite_protocol_trace_from_app_iff in Htr.
   destruct Htr as [Hepref Hesuf].
-  specialize (equivocate_trace_from_protocol_free _ Hreset_state _ _ (conj Hepref His))
+  specialize (replay_trace_from_protocol_free _ Hfull_replay_state _ _ (conj Hepref His))
     as Hepref_free.
   specialize (finite_ptrace_last_pstate _ _ _ Hepref_free) as Hlast_free.
   destruct (input eitem) as [m|] eqn:Hinput; [|exact I].
@@ -1022,7 +1022,7 @@ Proof.
   apply
     (specialized_selected_message_exists_in_some_traces_from (free_composite_vlsm equivocator_IM i0)
       output
-    ) with reset_state (equivocate_trace_from reset_state is epref)
+    ) with full_replay_state (replay_trace_from full_replay_state is epref)
   ; [assumption|reflexivity|].
   apply Exists_exists in Heqv.
   destruct Heqv as [mitem [Hmitem Houtput]].
@@ -1031,10 +1031,10 @@ Proof.
   change (mitem :: suf) with ([mitem] ++ suf) in Heqepref.
   subst epref.
   rewrite app_assoc.
-  rewrite equivocate_trace_from_app.
+  rewrite replay_trace_from_app.
   apply Exists_app. left.
   destruct
-    (equivocate_trace_from_state_correspondence' reset_state is His (pref ++ [mitem]) eqv)
+    (replay_trace_from_state_correspondence' full_replay_state is His (pref ++ [mitem]) eqv)
     as [_ [Houtput' _]].
   spec Houtput'.
   { intro contra; destruct pref; discriminate contra. }
@@ -1044,20 +1044,20 @@ Proof.
   rewrite trace_to_action_to_trace in Houtput'; [|assumption].
   change
     (fst (apply_action equivocators_no_equivocations_vlsm
-    reset_state
+    full_replay_state
     (spawn_initial_state is ++
      map
        (update_euivocators_transition_item_descriptor
-          reset_state) (pref ++ [mitem]))))
-    with (equivocate_trace_from reset_state is (pref ++ [mitem]))
+          full_replay_state) (pref ++ [mitem]))))
+    with (replay_trace_from full_replay_state is (pref ++ [mitem]))
     in Houtput'.
-  rewrite equivocate_trace_from_app.
-  rewrite equivocate_trace_from_app in Houtput'.
+  rewrite replay_trace_from_app.
+  rewrite replay_trace_from_app in Houtput'.
   apply Exists_app. right. simpl.
   rewrite last_error_is_last in Houtput'.
   simpl in Houtput'.
   unfold apply_action. unfold apply_action in Houtput'. simpl in *.
-  destruct (update_euivocators_transition_item_descriptor reset_state mitem) eqn:Hupdated_item.
+  destruct (update_euivocators_transition_item_descriptor full_replay_state mitem) eqn:Hupdated_item.
   simpl in *.
   match goal with
   |- context [vtransition ?V ?l ?som] =>
